src/program_proof/simplepb/pb_increasecommit_proof.v
@@ -1,0 +1,235 @@
+From Perennial.program_proof Require Import grove_prelude.
+From Goose.github_com.mit_pdos.gokv.simplepb Require Export pb.
+From Perennial.program_proof.simplepb Require Export pb_protocol.
+From Perennial.program_proof.simplepb Require Import pb_marshal_proof.
+From Perennial.program_proof Require Import marshal_stateless_proof.
+From Perennial.program_proof.simplepb Require Import pb_definitions.
+From Perennial.program_proof.reconnectclient Require Import proof.
+From RecordUpdate Require Import RecordSet.
+Import RecordSetNotations.
+
+Section pb_increasecommit_proof.
+Context `{!heapGS Σ}.
+Context {pb_record:Sm.t}.
+
+Notation OpType := (Sm.OpType pb_record).
+Notation has_op_encoding := (Sm.has_op_encoding pb_record).
+Notation has_snap_encoding := (Sm.has_snap_encoding pb_record).
+Notation compute_reply := (Sm.compute_reply pb_record).
+Notation pbG := (pbG (pb_record:=pb_record)).
+Notation own_Server_ghost_f := (own_Server_ghost_f (pb_record:=pb_record)).
+
+Context `{!waitgroupG Σ}.
+Context `{!pbG Σ}.
+
+Lemma wp_Clerk__IncreaseCommit γ γsrv ck (epoch:u64) (newCommitIndex:u64) σ :
+  {{{
+        "#Hck" ∷ is_Clerk ck γ γsrv ∗
+        "%HcommitLen" ∷ ⌜int.nat newCommitIndex = length σ⌝ ∗
+        "#Hghost_epoch_lb" ∷ is_epoch_lb γsrv.(r_pb) epoch ∗
+        "#Hcommit_by" ∷ committed_by γ.(s_pb) epoch σ ∗
+        "#Hlog_lb" ∷ is_pb_log_lb γ.(s_pb) σ
+  }}}
+    Clerk__IncreaseCommitIndex #ck #newCommitIndex
+  {{{ (err:u64), RET #err; True }}}.
+Proof.
+  iIntros (Φ) "Hpre HΦ".
+  iNamed "Hpre".
+  wp_call.
+  wp_apply (wp_ref_of_zero).
+  { done. }
+  iIntros (rep) "Hrep".
+  wp_pures.
+  iNamed "Hck".
+  wp_call.
+  replace (slice.nil) with (slice_val Slice.nil) by done.
+  wp_apply (wp_WriteInt with "[]").
+  { iApply is_slice_zero. }
+  iIntros (enc_args_sl) "Henc_args_sl".
+  wp_loadField.
+  iDestruct (is_slice_to_small with "Henc_args_sl") as "Henc_args_sl".
+  wp_apply (wp_frame_wand with "HΦ").
+  rewrite is_pb_host_unfold.
+  iNamed "Hsrv".
+  wp_apply (wp_ReconnectingClient__Call2 with "Hcl_rpc [] Henc_args_sl Hrep").
+  {
+    iDestruct "Hsrv" as "(_ & _ & _ & _ & _ & _& $ & _)".
+  }
+  { (* Successful RPC *)
+    iModIntro.
+    iNext.
+    unfold IncreaseCommit_spec.
+    repeat iExists _.
+    iSplitR; first done.
+    simpl.
+    unfold IncreaseCommit_core_spec.
+    iFrame "#%".
+    iIntros "_ %_ _ _ H".
+    by iApply "H".
+  }
+  {
+    iIntros (??) "_ _ H".
+    by iApply "H".
+  }
+Qed.
+
+(** Helper lemmas for GetState() server-side proof *)
+Lemma increase_commitIndex_step γ γsrv st committedOps :
+  no_overflow (length committedOps) →
+  is_pb_log_lb γ.(s_pb) committedOps -∗
+  is_proposal_lb γ.(s_pb) st.(server.epoch) committedOps -∗
+  committed_by γ.(s_pb) st.(server.epoch) committedOps -∗
+  own_Server_ghost_eph_f st γ γsrv
+  ={↑pbN}=∗
+  own_Server_ghost_eph_f (st <| server.committedNextIndex := length committedOps |> ) γ γsrv
+.
+Proof.
+  iIntros (?) "#Hghost_lb #Hprop_lb #Hcomm_by".
+  rewrite /own_Server_ghost_eph_f /tc_opaque /=.
+  iNamed 1.
+  rewrite /own_Primary_ghost_f /tc_opaque /=.
+  iNamed "Hprimary".
+  repeat iExists _; iFrame "Hghost_lb ∗ #".
+  iPureIntro.
+  split; first done.
+  rewrite /get_rwops fmap_length /=.
+  by unfold no_overflow in H.
+Qed.
+
+Lemma wp_Server__IncreaseCommit γ γsrv s args newCommitIndex Φ Ψ :
+  is_Server s γ γsrv -∗
+  (∀ reply, Ψ reply -∗ ∀ (reply_ptr:loc), GetStateReply.own reply_ptr reply -∗ Φ #reply_ptr) -∗
+  IncreaseCommit_core_spec γ γsrv args.(GetStateArgs.epoch) epoch_lb Ψ -∗
+  WP pb.Server__IncreaseCommitIndex #s #newCommitIndex {{ Φ }}
+  .
+Proof.
+  iIntros "His_srv Hargs HΦ HΨ".
+  wp_call.
+  iNamed "His_srv".
+  wp_loadField.
+  wp_apply (acquire_spec with "HmuInv").
+  iIntros "[Hlocked Hown]".
+  iNamed "Hown".
+  wp_pures.
+  iNamed "Hargs".
+  wp_loadField.
+  iNamed "Hvol".
+  wp_loadField.
+  wp_if_destruct.
+  { (* reply with error *)
+    wp_loadField.
+    wp_apply (release_spec with "[-HΦ HΨ]").
+    {
+      iFrame "HmuInv Hlocked".
+      iNext.
+      repeat (iExists _).
+      iSplitR "HghostEph"; last iFrame.
+      repeat (iExists _).
+      iFrame "∗#%".
+    }
+    unfold GetState_core_spec.
+    iDestruct "HΨ" as "[_ HΨ]".
+    iRight in "HΨ".
+    wp_pures.
+    iDestruct (is_slice_small_nil byteT 1 Slice.nil) as "#Hsl_nil".
+    { done. }
+    iMod (readonly_alloc_1 with "Hsl_nil") as "Hsl_nil2".
+    wp_apply (wp_allocStruct).
+    { Transparent slice.T. repeat econstructor.
+      Opaque slice.T. }
+    iIntros (reply_ptr) "Hreply".
+    iDestruct (struct_fields_split with "Hreply") as "HH".
+    iNamed "HH".
+    iApply ("HΦ" with "[HΨ]"); last first.
+    {
+      iExists _. iFrame.
+      instantiate (1:=GetStateReply.mkC _ _ _).
+      replace (slice.nil) with (slice_val Slice.nil) by done.
+      iFrame.
+    }
+    simpl.
+    iApply "HΨ".
+    done.
+  }
+  wp_storeField.
+  wp_loadField.
+
+  iDestruct (is_StateMachine_acc_getstate with "HisSm") as "HH".
+  iNamed "HH".
+  wp_loadField.
+  iDestruct "HΨ" as "[#Hepoch_lb HΨ]".
+  iDestruct (getstate_eph with "HghostEph") as "HghostEph".
+  wp_apply ("HgetstateSpec" with "[$Hstate]").
+  {
+    iIntros "Hghost".
+    iMod (getstate_step with "Hepoch_lb Hghost") as "[Hghost HH]".
+    iFrame "Hghost".
+    iModIntro.
+    iExact "HH".
+  }
+  iIntros (??) "(#Hsnap_sl & %Hsnap_enc & [Hstate HQ])".
+  iDestruct "HQ" as (?) "(%Hσeq_phys & #Hacc_ro &  #Hprop_lb & #Hprop_facts & #Hprim_facts & %Hepoch_ineq)".
+  wp_pures.
+  wp_loadField.
+  wp_pures.
+  wp_loadField.
+
+  iLeft in "HΨ".
+  iDestruct ("HΨ" with "[% //] [%] Hacc_ro Hprop_facts Hprim_facts Hprop_lb [%] [%]") as "HΨ".
+  { word. }
+  { rewrite -Hσeq_phys. done. }
+  { apply (f_equal length) in Hσeq_phys.
+    unfold no_overflow in HnextIndexNoOverflow. (* FIXME: why manually unfold? *)
+    word. }
+
+  (* signal all opApplied condvars *)
+  wp_apply (wp_MapIter with "HopAppliedConds_map HopAppliedConds_conds").
+  { iFrame "HopAppliedConds_conds". }
+  { (* prove one iteration of the map for loop *)
+    iIntros.
+    iIntros (?) "!# [_ #Hpre] HΦ".
+    wp_pures.
+    wp_apply (wp_condSignal with "Hpre").
+    iApply "HΦ".
+    iFrame "#".
+    instantiate (1:=(λ _ _, True)%I).
+    done.
+  }
+  iIntros "(HopAppliedConds_map & _ & _)".
+
+  wp_pures.
+  wp_apply (wp_NewMap).
+  iIntros (opAppliedConds_loc_new) "Hmapnew".
+  wp_storeField.
+  wp_loadField.
+  wp_apply (wp_condBroadcast with "[]").
+  { done. }
+  wp_loadField.
+  wp_apply (release_spec with "[-Hsnap_sl HΨ HΦ]").
+  {
+    iFrame "HmuInv Hlocked".
+    iNext.
+    repeat (iExists _).
+    iFrame "HghostEph".
+    repeat (iExists _).
+    iFrame "∗ HisSm #".
+    iFrame "%".
+    by iApply big_sepM_empty.
+  }
+  wp_apply (wp_allocStruct).
+  { Transparent slice.T. repeat econstructor.
+    Opaque slice.T. }
+  iIntros (reply_ptr) "Hreply".
+  iDestruct (struct_fields_split with "Hreply") as "HH".
+  iNamed "HH".
+  iApply ("HΦ" with "HΨ").
+  iExists _.
+  iFrame.
+  simpl.
+
+  apply (f_equal length) in Hσeq_phys.
+  rewrite Hσeq_phys.
+  iFrame "∗#".
+Qed.
+
+End pb_increasecommit_proof.
